\documentclass[11pt]{jarticle}
\input{A4}
\usepackage{graphics}
\usepackage{amssymb}
\usepackage{marvosym}

\usepackage{theorem}
\newtheorem{assumption}{Assumption}

\renewcommand{\baselinestretch}{1.15}
\setlength{\parskip}{0.5ex}
\renewcommand{\arraystretch}{0.8}

\begin{document}

\section{Evaluation of polynomial}

Let $A(x) = a_0 + a_1 x^1 + a_2 x^2 + \cdots + a_{n-1} x^{n-1}$ be a polynomial of degree $(n-1)$ , and 
let $a = (a_0, a_1, \ldots, a_{n-1})$ be the coefficient array of $A$. 

We assume that, without loss of generality, $n$ is an even number. 
(If not, let $n' = n + 1$ and consider $A'$ such that $a' = (a_0, a_1, \ldots, a_{n-1}, 0)$.)
Then we have
\begin{eqnarray*}
A(x) &=& a_0 + a_2 x^2 + \cdots + a_{n-2} x^{n-2}
+ a_1 x^1 + a_3 x^3 + \cdots +a_{n-1} x^{x-1} \\
&=& \sum_{i=0}^{n/2 - 1} a_{2i} x^{2i} + x \cdot\sum_{i=0}^{n/2 - 1} a_{2i+1} x^{2i} \,.
\end{eqnarray*}
By introducing two polynomial coefficient arrays of $A_0$ with $(a_0, a_2, \ldots, a_{n-2})$ and $A_1$ with $(a_1, a_3, \ldots, a_{n-1})$, the above can be rewritten to 
\begin{eqnarray*}
A(x) = A_0(x^2) + x A_1(x^2) \,.
\end{eqnarray*}

Therefore, if we calcurate $\log{n}$ terms $x^2, x^4, \ldots, x^{n/2}$, time complexity $T(n)$ to obtain the value $A(x)$ of polynomial degree $n-1$ is 
\[
T(n) =
\left\{\begin{array}{ll}
2 & n \leq 1 \\
2T(n/2) + 2 & \mbox{otherwise.}
\end{array}\right.
\]

\section{String matching}

Let $\Sigma$ be a finite alphabet, $t$ a text $t = t_0 \cdot t_1 \cdot \cdots\cdot t_{n-1}$ over $\Sigma^*$, 
and $p$ a pattern string $p \in \Sigma^*$. 

Let $\omega^{i}$ be a coefficient in $\mathbb{C}$. 
We define a text and a pattern in complex vector  
\begin{eqnarray*}
T(i) = t_i \cdot \omega^{n-1-i}, \\
P(i) = p_i \cdot w_p^{i}
\end{eqnarray*}
where 
\begin{eqnarray*}
w_p^i = \left\{\begin{array}{ll}
\omega^i & 0 \leq i < |p|\\
0 & i \geq |p|
\end{array}\right. .
\end{eqnarray*}

\begin{eqnarray*}
M(i) = \sum_{k = 0}^{n-1} T(i+k) \cdot P(k) = \sum_{k=0}^{k < |p|} t_{i+k} \cdot p_i \cdot \omega^{n-1-(i+k)+k}
= \sum_{k = 0}^{k < |p|}  t_{i+k} \cdot p_i \cdot \omega^{n-1-i}
\end{eqnarray*}

For $t = t_0 \cdot t_1 \cdot t_2 \cdot t_3 \cdot t_4 \cdots t_{n-1}$ and $p = p_0 \cdot p_1 \cdot p_2$, 
we examine whether $p$ occurs at position $2$ by 
$M(2) = t_2 p_0 \omega^{n-1-2 + 0}+ t_3 p_1 \omega^{n-1-3 + 1} + t_4 p_2 \omega^{n-1-4 + 2}$, thus $M(2) = \omega^{n-1-3}(t_2 p_0 + t_3 p_1 + t_4 p_2)$. 


\end{document}